theories/common/ConcRA.v
@@ -44,6 +44,10 @@ Section preds.
       ((λ x, if (decide (x = tid)) then Some (Excl ()) else None) : nat -d> optionUR (exclR unitO)).
   Arguments YieldToken : simpl never.
 
+  Definition YieldTokenAuth (nths: nat) : iProp Σ :=
+    Seal.sealing "Conc" own base_γ
+      ((λ x, if (decide (x <= nths)) then None else Some (Excl ())) : nat -d> optionUR (exclR unitO)).
+
   Lemma YieldToken_both tid0 tid1 : YieldToken tid0 -∗ YieldToken tid1 -∗ ⌜tid0 ≠ tid1⌝.
   Proof.
     rewrite /YieldToken; unseal "Conc".
@@ -54,3 +58,4 @@ End preds.
 
 Notation "'TID' tid" := (TidToken tid) (at level 20, tid at level 1, format "TID  tid").
 Notation "'YIELD' tid" := (YieldToken tid) (at level 20, tid at level 1, format "YIELD  tid").
+
